[conn] Use single tag for all messages.

examples/conn/impl.v
@@ -14,19 +14,22 @@ Unset Printing Implicit Defensive.
 Notation connN := (nroot.@"conn").
 
 Definition channel : val := λ: "cs",
-  Snd "cs".
+  Snd (Fst "cs").
 
-Definition sent     : val := λ: "cs", Fst (Fst "cs") +ₗ #0%nat.
-Definition received : val := λ: "cs", Fst (Fst "cs") +ₗ #1%nat.
+Definition sent     : val := λ: "cs", Fst (Fst (Fst "cs")) +ₗ #0%nat.
+Definition received : val := λ: "cs", Fst (Fst (Fst "cs")) +ₗ #1%nat.
 
 Definition session_key : val := λ: "cs",
-  Snd (Fst "cs").
+  Snd (Fst (Fst "cs")).
+
+Definition role : val := λ: "cs",
+  Snd "cs".
 
 Definition connect : val := λ: "c" "skA" "pkB" "N",
   let: "session_key" :=
     do_until (λ: <>, initiator "c" "skA" "pkB" "N") in
   let: "counters" := AllocN #2 #0%nat in
-  ("counters", "session_key", "c").
+  ("counters", "session_key", "c", #1).
 
 Definition listen : val := λ: "c",
   responder_wait "c".
@@ -37,46 +40,35 @@ Definition confirm : val := λ: "c" "skB" "N" "req",
   let: "sk" := do_until
     (λ: <>, responder_accept "c" "skB" "ga" "pkA" "N") in
   let: "counters" := AllocN #2 #0%nat in
-  let: "conn" := ("counters", "sk", "c") in
+  let: "conn" := ("counters", "sk", "c", #0) in
   "conn".
 
-Definition send : val := λ: "cs" "N" "ts",
+Definition send : val := λ: "cs" "t",
   let: "c"  := channel "cs" in
   let: "n"  := sent "cs" in
   let: "sk" := session_key "cs" in
-  let: "m"  := term_of_list (tint !"n" :: "ts") in
-  let: "m"  := senc "sk" "N" "m" in
+  let: "m"  := term_of_list [tint (role "cs"); tint !"n"; "t"] in
+  let: "m"  := senc "sk" (Tag connN) "m" in
   send "c" "m";;
   "n" <- !"n" + #1%nat.
 
-Definition try_open : val := λ: "cs" "N" "t",
-  bind: "t" := untag "N" "t" in
-  bind: "ts" := list_of_term "t" in
-  let: "m" := !(received "cs") in
-  match: "ts" with
-    NONE => NONE
-  | SOME "ts" =>
-    bind: "m'" := to_int (Fst "ts") in
-    guard: "m" = "m'" in
-    received "cs" <- "m" + #1;;
-    SOME (Snd "ts")
-  end.
-
-Definition handle : val := λ: "N" "handler" "cs" "t",
-  bind: "ts" := try_open "cs" "N" "t" in
-  SOME ("handler" "cs" "ts").
-
-Definition select : val := λ: "cs" "handlers",
+Definition recv : val := λ: "cs",
+  let: "c"  := channel "cs" in
+  let: "rl" := role "cs" in
   let: "sk" := session_key "cs" in
   do_until (λ: <>,
-    let: "t" := recv (channel "cs") in
-    bind: "t" := open "sk" "t" in
-    scan_list (λ: "handler", "handler" "cs" "t") "handlers").
-
-Definition recv : val :=
-  λ: "cs" "N", select "cs" [handle "N" (λ: <> "ts", "ts")%E].
+    let: "t" := recv "c" in
+    let: "r" := received "cs" in
+    bind: "t" := sdec "sk" (Tag connN) "t" in
+    bind: "t" := list_of_term "t" in
+    list_match: ["rl'"; "r'"; "t"] := "t" in
+    bind: "rl'" := to_int "rl'" in
+    bind: "r'" := to_int "r'" in
+    guard: ("rl" ≠ "rl'") && (!"r" = "r'") in
+    "r" <- !"r" + #1;;
+    SOME "t").
 
 Definition free : val := λ: "cs",
-  let: "counters" := Fst (Fst "cs") in
+  let: "counters" := Fst (Fst (Fst "cs")) in
   Free "counters";;
   Free ("counters" +ₗ #1%nat).
