examples/conn/proofs/base.v
@@ -7,6 +7,7 @@ From iris.heap_lang Require Import notation proofmode.
 From iris.heap_lang.lib Require Import ticket_lock.
 From cryptis Require Import lib term gmeta nown.
 From cryptis Require Import cryptis primitives tactics role.
+From cryptis Require Import saved_prop.
 From cryptis.examples Require Import iso_dh.
 
 Set Implicit Arguments.
@@ -26,18 +27,21 @@ Definition cs_share cs := si_share_of (cs_role cs) cs.
 
 #[global]
 Instance cs_repr : Repr state :=
-  λ s, (#(cs_ts s), si_key s, cs_chan s)%V.
+  λ s, (#(cs_ts s), si_key s, cs_chan s, repr (cs_role s))%V.
 
 Definition countR := authR max_natUR.
 
 Class connGS Σ := ConnGS {
   connGS_count  : inG Σ countR;
+  connGS_pred   : savedPredG Σ (sign_key * sign_key * sess_info * role * term);
 }.
 
 Local Existing Instance connGS_count.
+Local Existing Instance connGS_pred.
 
 Definition connΣ := #[
-  GFunctor countR
+  GFunctor countR;
+  savedPredΣ (sign_key * sign_key * sess_info * role * term)
 ].
 
 Global Instance subG_connGS Σ : subG connΣ Σ → connGS Σ.
@@ -56,6 +60,8 @@ Implicit Types b : bool.
 Implicit Types v : val.
 Implicit Types (ok : Prop) (failed : bool).
 Implicit Types si : sess_info.
+Implicit Types (φ : sign_key → sign_key → sess_info → role → term → iProp).
+Implicit Types (ψ : role → term → iProp).
 
 Definition failure skI skR : iProp :=
    public skI ∨ public skR.
@@ -119,21 +125,32 @@ iInv nroot as "[HP|>recv']".
   case: valid => /= ? _; lia.
 Qed.
 
-Definition connected skI skR rl cs : iProp :=
+Definition conn_msg_pred φ gb : iProp :=
+  □ (∀ si rl t,
+        term_pred gb (iso_dhN.@"res".@"pred")
+          (si_init si, si_resp si, si, rl, t)
+          ↔ ▷ φ (si_init si) (si_resp si) si rl t).
+
+Definition conn_init_pred φ ψ gb : iProp :=
+  conn_msg_pred φ gb ∗ ψ Init gb.
+
+Definition connected skI skR φ rl cs : iProp :=
   ⌜si_init cs = skI⌝ ∗
   ⌜si_resp cs = skR⌝ ∗
   ⌜cs_role cs = rl⌝ ∗
   channel (cs_chan cs) ∗
   wf_sess_info (cs_role cs) cs ∗
+  (compromised_session rl cs ∨
+     conn_msg_pred φ (si_resp_share cs)) ∗
   ∃ n m, cs_ts cs ↦∗ [ #n; #m ] ∗ received_auth cs (cs_role cs) m.
 
-Lemma connected_channel skI skR rl cs :
-  connected skI skR rl cs -∗
+Lemma connected_channel skI skR φ rl cs :
+  connected skI skR φ rl cs -∗
   channel (cs_chan cs).
 Proof. by iIntros "(_ & _ & _ & ? & _)". Qed.
 
-Lemma connected_public_key skI skR rl cs :
-  connected skI skR rl cs -∗
+Lemma connected_public_key skI skR φ rl cs :
+  connected skI skR φ rl cs -∗
   release_token (si_share_of rl cs) -∗
   public (si_key cs) -∗
   ◇ compromised_session rl cs.
@@ -144,45 +161,74 @@ iDestruct "sess" as "(#? & #sess)".
 by iApply (session_compromised with "[] [//] rel").
 Qed.
 
-Lemma connected_released_session skI skR rl cs :
-  connected skI skR rl cs -∗
+Lemma connected_released_session skI skR φ rl cs :
+  connected skI skR φ rl cs -∗
   □ (▷ released_session cs → public (si_key cs)).
 Proof.
 iIntros "(_ & _ & _ & _ & #sess & _)".
 by iDestruct "sess" as "(_ & ? & sess)".
 Qed.
 
-Lemma connected_keyE skI skR rl cs :
-  connected skI skR rl cs -∗
+Lemma connected_keyE skI skR φ rl cs :
+  connected skI skR φ rl cs -∗
   ⌜skI = si_init cs⌝ ∗ ⌜skR = si_resp cs⌝ ∗ ⌜rl = cs_role cs⌝.
 Proof. by iIntros "(-> & -> & -> & _)". Qed.
 
-Lemma connected_ok skI skR rl cs :
-  connected skI skR rl cs -∗
+Lemma connected_ok skI skR φ rl cs :
+  connected skI skR φ rl cs -∗
   secret skI -∗
   secret skR -∗
   minted skI -∗
   minted skR -∗
   ◇ □ ¬ compromised_session rl cs.
 Proof.
-iIntros "(<- & <- & <- & _ & #sess & % & % & _ & _) s_kI s_kR #signI #signR".
+iIntros "(<- & <- & <- & _ & #sess & _ & % & % & _ & _)
+          s_kI s_kR #signI #signR".
 iDestruct "sess" as "(m_k & sess)".
 by iApply (session_not_compromised with "[//] s_kI s_kR").
 Qed.
 
-Definition conn_pred rl φ kS t : iProp :=
-  ∃ si n ts,
+Definition conn_pred kS t : iProp :=
+  ∃ si rl n t',
+    let rl' := TInt (if rl is Init then 1 else 0) in
     ⌜kS = si_key si⌝ ∗
-    ⌜t = Spec.of_list (TInt n :: ts)⌝ ∗
-    ([∗ list] t' ∈ ts, public t') ∗
-    escrow nroot
-      (received_auth si (swap_role rl) n)
-      (φ (si_init si) (si_resp si) si ts ∗
-       received_auth si (swap_role rl) (S n)).
+    ⌜t = Spec.of_list [rl'; TInt n; t']⌝ ∗
+    public t' ∗
+    escrow nroot (received_auth si (swap_role rl) n)
+      (term_pred (si_resp_share si) (iso_dhN.@"res".@"pred")
+         (si_init si, si_resp si, si, rl, t')
+       ∗ received_auth si (swap_role rl) (S n)).
 
 Lemma session_failed_failure rl si :
   compromised_session rl si  ⊢ failure (si_init si) (si_resp si).
 Proof. by iIntros "(#failed & _)". Qed.
+
+Definition pre_ctx `{!iso_dhGS Σ} : iProp :=
+  iso_dh_ctx ∗
+  senc_pred connN conn_pred.
+
+Lemma pre_ctx_alloc `{!iso_dhGS Σ} E :
+  ↑connN ⊆ E →
+  iso_dh_ctx -∗
+  seal_pred_token SENC E ==∗
+  pre_ctx ∗ seal_pred_token SENC (E ∖ ↑connN).
+Proof.
+iIntros "% #? tok". iFrame "#". by iApply seal_pred_set.
+Qed.
+
+Definition ctx `{!iso_dhGS Σ} N φ ψ : iProp :=
+  pre_ctx ∗
+  iso_dh_pred N (conn_init_pred φ ψ).
+
+Lemma ctx_alloc `{!iso_dhGS Σ} N φ ψ E :
+  ↑N ⊆ E →
+  pre_ctx -∗
+  iso_dh_token E ==∗
+  ctx N φ ψ ∗ iso_dh_token (E ∖ ↑N).
+Proof.
+iIntros "% #ctx tok". iFrame "#".
+by iApply iso_dh_pred_set.
+Qed.
 
 End Defs.
 
