examples/rpc/proofs.v
@@ -13,6 +13,12 @@ Set Implicit Arguments.
 Unset Strict Implicit.
 Unset Printing Implicit Defensive.
 
+Record handler := Handler {
+  handler_val : val;
+}.
+
+Instance repr_handler : Repr handler := handler_val.
+
 Section Proofs.
 
 Context `{!cryptisGS Σ, !heapGS Σ, !iso_dhGS Σ, !Conn.connGS Σ, !rpcGS Σ}.
@@ -38,11 +44,8 @@ Lemma wp_connect P c skI skR :
       client_connected skI skR cs ∗
       (compromised_session Init cs ∨ P) }}}.
 Proof.
-iIntros "#? #? #? #? #? % !> P post".
-wp_lam; wp_pures.
-iPoseProof (ctx_iso_dh_ctx with "[//]") as "?".
-iPoseProof (ctx_iso_dh_pred with "[//]") as "?".
-iApply wp_fupd.
+iIntros "#? #? [#? #?] #? #? % !> P post".
+wp_lam; wp_pures. iApply wp_fupd.
 wp_apply (Conn.wp_connect with "[] [P]"); eauto 10.
 iIntros "%cs (connected & P & rel & token)".
 rewrite bi.sep_True.
@@ -60,9 +63,8 @@ Lemma wp_listen c :
   {{{ ga skI, RET (ga, Spec.pkey skI)%V;
       public ga ∗ minted skI }}}.
 Proof.
-iIntros "#? #? #? % !> _ post".
-wp_lam. iApply Conn.wp_listen => //.
-by iApply ctx_iso_dh_ctx.
+iIntros "#? #? [#? #?] % !> _ post".
+wp_lam. by iApply Conn.wp_listen.
 Qed.
 
 Lemma wp_confirm P c skI skR ga :
@@ -76,91 +78,175 @@ Lemma wp_confirm P c skI skR ga :
       server_connected skI skR cs ∗
       (compromised_session Resp cs ∨ P) }}}.
 Proof.
-iIntros "#? #ctx #? !> %Φ (#p_ga & #m_skI & #m_skR & P) post".
-wp_lam; wp_pures.
-iPoseProof (ctx_iso_dh_ctx with "[//]") as "?".
-iPoseProof (ctx_iso_dh_pred with "[//]") as "?".
-iApply wp_fupd.
-wp_apply (Conn.wp_confirm P (λ _, True)%I with "[//] [//] [//] [//] [$P]").
+iIntros "#? #ctx1 [#? #ctx2] !> %Φ (#p_ga & #m_skI & #m_skR & P) post".
+wp_lam; wp_pures. iApply wp_fupd.
+wp_apply (Conn.wp_confirm P (λ _ _, True)%I with "[//] [//] ctx2 [$P]").
 { do !iSplit => //. by iIntros "!> % _ !>". }
 iIntros "%cs (conn & dis & rel & token & _)".
 iApply "post". by iFrame.
 Qed.
 
-Lemma wp_call N φ ψ skI skR cs (ts : list term) :
-  {{{ cryptis_ctx ∗ ctx ∗
-      ([∗ list] t ∈ ts, public t) ∗
-      rpc N φ ψ ∗
+Lemma wp_call N φ ψ skI skR cs t :
+  {{{ cryptis_ctx ∗ ctx ∗ public t ∗
+      rpc_pred N φ ψ ∗
       client_connected skI skR cs ∗
-      (compromised_session Init cs ∨ φ skI skR cs ts) }}}
-    impl.call (repr cs) (Tag N) (repr ts)
-  {{{ ts', RET (repr ts');
+      (compromised_session Init cs ∨ φ skI skR cs t) }}}
+    impl.call (repr cs) (Tag N) t
+  {{{ t', RET (repr t');
       client_connected skI skR cs ∗
-      (compromised_session Init cs ∨ ψ skI skR cs ts ts') ∗
-      ([∗ list] t ∈ ts', public t) }}}.
+      (compromised_session Init cs ∨ ψ skI skR cs t t') ∗
+      public t' }}}.
 Proof.
-iIntros "%Φ (#? & #? & #p_ts & #? & conn & inv) post".
+iIntros "%Φ (#? & #ctx & #p_t & #N & conn & inv) post".
+iDestruct "ctx" as "[? ctx]".
 iDestruct "conn" as "(conn & rel & resp_pred)".
 iAssert (|==>
-  (compromised_session Init cs ∨ resp_pred_token cs (ψ skI skR cs ts)) ∗
+  (compromised_session Init cs ∨ resp_pred_token cs N t) ∗
   (compromised_session Init cs ∨
-     resp_pred_token cs (ψ skI skR cs ts) ∗
-     φ skI skR cs ts))%I
+     resp_pred_token cs N t ∗ φ skI skR cs t))%I
   with "[resp_pred inv]" as ">[resp_pred inv]".
 { rewrite -or_sep2.
   iDestruct "resp_pred" as "[#fail|(t1 & t2)]"; eauto.
-  iMod (resp_pred_token_update _ _ _ (ψ skI skR cs ts)
-         with "t1 t2") as "[t1 t2]".
+  iMod (resp_pred_token_update cs N t with "t1 t2") as "[t1 t2]".
   iDestruct "inv" as "[#fail|inv]"; eauto.
   iModIntro. iRight. by iFrame. }
-wp_lam. wp_pure _ credit:"c". wp_pures.
+wp_lam. wp_pure _ credit:"c". wp_pures. wp_tag.
 wp_apply (Conn.wp_send with "[] [] [$conn inv]"); eauto.
-{ iDestruct "inv" as "[(_ & ? & _)|inv]"; first by eauto. iRight.
-  by iFrame. }
+{ by rewrite public_tag. }
+{ iDestruct "inv" as "[(_ & ? & _)|[??]]"; first by eauto. iRight.
+  iExists N, t, φ, ψ. iSplit => //. by iFrame. }
 iIntros "conn". wp_pures. iApply wp_fupd.
 wp_apply (Conn.wp_recv with "[] [$conn]"); eauto.
-{ by iApply ctx_resp. }
-iIntros "%ts' (conn & p_ts' & inv)".
+iIntros "%t' (conn & p_t' & inv)".
 iApply "post".
 iDestruct "inv" as "[#inv|inv]".
 { iPoseProof (Conn.connected_public_key with "conn rel [//]") as "#>?".
   iFrame. iModIntro. iSplitL; by eauto. }
 iDestruct "resp_pred" as "[#fail|t1]".
 { iFrame. iModIntro. iSplitL; eauto. }
-iDestruct "inv" as "(%ψ' & t2 & inv)".
-iPoseProof (resp_pred_token_agree with "t1 t2") as "#E".
-iSpecialize ("E" $! ts').
+iDestruct "inv" as "(%N' & %t₀ & %φ' & %ψ' & #N' & inv & t2)".
+iPoseProof (resp_pred_token_agree with "t1 t2") as "[<- <-]".
+iPoseProof (rpc_pred_agree with "N N'") as "[_ E]".
 iMod (lc_fupd_elim_later_pers with "c E") as "{E} #E".
-iRewrite "E".
-iMod (resp_pred_token_update _ _ _ (λ _, False%I)
-       with "t1 t2") as "ts".
+iRewrite ("E" $! skI skR cs t t').
+iMod (resp_pred_token_update _ rpcN (TInt 0)
+       with "t1 t2") as "t".
 by iFrame.
 Qed.
 
-Definition wf_handler Φ skI skR cs h : iProp :=
-  Conn.wf_handler
-    (release_token (si_resp_share cs) ∗ Φ)%I
-    (λ r,
-      ⌜r = #true⌝ ∗ Φ ∗
-      Conn.connected skI skR Resp cs ∗
-      release_token (si_resp_share cs) ∨
-      ⌜r = #false⌝ ∗ Φ ∗
-      public (si_key cs))%I
-    skI skR Resp cs h.
+(* TODO *)
+#[global] Instance repr_bool : Repr bool := λ b, #b.
 
-Lemma wp_handle Φ N φ₁ φ₂ skI skR cs (f : val) :
+Definition wf_handler Φ skI skR cs (h : handler) : iProp :=
+  □ ∀ t,
+    {{{ public t ∗
+        (public (si_key cs) ∨ rpc_msg_pred skI skR cs Init t) ∗
+        server_connected skI skR cs ∗
+        Φ }}}
+      repr h (repr cs) t
+    {{{ ob, RET (repr ob);
+        match ob : option bool with
+        | Some true =>
+            Φ ∗ server_connected skI skR cs
+        | Some false => Φ ∗ public (si_key cs)
+        | None =>
+            Φ ∗ server_connected skI skR cs ∗
+            (public (si_key cs) ∨ rpc_msg_pred skI skR cs Init t)
+        end
+    }}}.
+
+Typeclasses Opaque wf_handler.
+
+Instance persistent_wf_handler Φ skI skR cs h :
+  Persistent (wf_handler Φ skI skR cs h).
+Proof. rewrite /wf_handler. apply _. Qed.
+
+Lemma wp_handle_gen Φ N φ ψ skI skR cs (f : val) :
   {{{
-    rpc N φ₁ φ₂ ∗
+    rpc_pred N φ ψ ∗
     ctx ∗
-    □ (∀ (ts : list term),
-      {{{ ▷ ([∗ list] t ∈ ts, public t) ∗
-          ▷ (compromised_session Resp cs ∨ φ₁ skI skR cs ts) ∗
+    □ (∀ t : term,
+      {{{ ▷ public t ∗
+          ▷ (compromised_session Resp cs ∨ φ skI skR cs t) ∗
+          release_token (si_resp_share cs) ∗
           Φ }}}
-        f (repr ts)
-      {{{ ts', RET (repr ts');
-          match ts' with
-          | Some ts' => ([∗ list] t ∈ ts', public t) ∗
-                        (compromised_session Resp cs ∨ φ₂ skI skR cs ts ts')
+        f (repr t)
+      {{{ ores, RET (repr ores);
+          match ores : option (bool * term) with
+          | Some (continue, t') =>
+              public t' ∗
+              if continue then
+                (compromised_session Resp cs ∨ ψ skI skR cs t t') ∗
+                release_token (si_resp_share cs)
+              else compromised_session Resp cs ∨ released_session cs
+          | None => release_token (si_resp_share cs)
+          end ∗
+          Φ }}})
+  }}}
+    impl.handle_gen (Tag N) f
+  {{{ h, RET (repr h); wf_handler Φ skI skR cs h }}}.
+Proof.
+iIntros "%Ξ (#N & #ctx & #wp) post". wp_lam. wp_pures.
+iDestruct "ctx" as "(#? & #?)".
+iIntros "!>". iApply ("post" $! (Handler _)). clear Ξ.
+rewrite /wf_handler.
+iIntros "!> %t !> %Ξ (#p_t & inv_t & (conn & rel) & inv) post".
+wp_pures. wp_untag t; wp_pures; last by iApply ("post" $! None); iFrame.
+iAssert (▷ (
+  Conn.connected skI skR rpc_msg_pred Resp cs ∗
+  release_token (si_resp_share cs) ∗
+  (compromised_session Resp cs ∨
+     resp_pred_token cs N t ∗ φ skI skR cs t)))%I
+  with "[conn rel inv_t]" as "(conn & >rel & inv_t)".
+{ iDestruct "inv_t" as "[#fail|inv_t]".
+  { iPoseProof (Conn.connected_public_key with "conn rel fail") as "#>?".
+    iFrame. by eauto. }
+  iFrame.
+  iDestruct "inv_t" as "(%N' & %t' & %φ' & %ψ' & %e & #N' & inv_t & token)".
+  case/Spec.tag_inj: e => /Tag_inj <- <- {N' t'}.
+  iPoseProof (rpc_pred_agree with "N N'") as "[E _]".
+  iModIntro. iRewrite ("E" $! skI skR cs t). iRight. iFrame. }
+rewrite public_tag.
+rewrite or_sep2. iDestruct "inv_t" as "[t inv_t]".
+wp_apply ("wp" with "[$inv $rel inv_t]").
+{ iSplit => //. }
+iIntros ([[continue t']|]) "[res inv]"; wp_pures; last first.
+{ by iApply ("post" $! (Some true)); iFrame. }
+iDestruct "res" as "(#p_t' & inv_t')".
+iPoseProof (Conn.connected_released_session with "conn") as "#sess".
+iAssert ((if continue then (compromised_session Resp cs ∨ ψ skI skR cs t t')
+          else public (si_key cs)) ∗
+         (if continue then release_token (si_resp_share cs) else public (si_key cs)))%I
+  with "[inv_t']" as "[inv_t' rel]".
+{ case: continue; eauto.
+  iDestruct "inv_t'" as "[(_&?&_)|inv_t']"; eauto.
+  iSplit; iApply "sess"; eauto. }
+wp_apply (Conn.wp_send with "[] p_t' [$conn t inv_t']"); eauto.
+{ iDestruct "t" as "[(_ & ? & _)|t]"; eauto.
+  case: continue; eauto.
+  iDestruct "inv_t'" as "[(_ & ? & _)|inv_t']"; eauto.
+  iRight. iExists _, _, _, _. iFrame. by iFrame "#". }
+iIntros "conn". wp_pures.
+case: continue; wp_pures.
+- by iApply ("post" $! (Some true)); iFrame.
+- wp_apply (Conn.wp_free with "conn"). iIntros "_". wp_pures.
+  iApply ("post" $! (Some false)). by eauto.
+Qed.
+
+Lemma wp_handle Φ N φ ψ skI skR cs (f : val) :
+  {{{
+    rpc_pred N φ ψ ∗
+    ctx ∗
+    □ (∀ t : term,
+      {{{ ▷ public t ∗
+          ▷ (compromised_session Resp cs ∨ φ skI skR cs t) ∗
+          Φ }}}
+        f (repr t)
+      {{{ ot', RET (repr ot');
+          match ot' : option term with
+          | Some t' =>
+              public t' ∗
+              (compromised_session Resp cs ∨ ψ skI skR cs t t')
           | None => True
           end ∗
           Φ }}})
@@ -168,39 +254,14 @@ Lemma wp_handle Φ N φ₁ φ₂ skI skR cs (f : val) :
     impl.handle (Tag N) f
   {{{ h, RET (repr h); wf_handler Φ skI skR cs h }}}.
 Proof.
-iIntros "%Ψ (#? & #ctx & #wp_f) post".
-iPoseProof (ctx_error with "[//]") as "#?".
-wp_lam; wp_pures.
-iApply Conn.wp_handle; last by eauto.
-iSplit => //. clear Ψ.
-iIntros "!> %ts !> %Ψ (conn & I & #p_ts & inv_ts) post".
-iDestruct "I" as "(rel & I)". wp_pures.
-iAssert (Conn.connected skI skR Resp cs ∗
-         release_token (si_resp_share cs) ∗
-         ◇ (compromised_session Resp cs ∨
-              resp_pred_token cs (φ₂ skI skR cs ts) ∗
-              φ₁ skI skR cs ts))%I
-  with "[conn rel inv_ts]" as "(conn & rel & >inv_ts)".
-{ iDestruct "inv_ts" as "[#fail|inv_ts]"; last by iFrame.
-  iPoseProof (Conn.connected_public_key with "conn rel [//]") as "#H".
-  iFrame. iMod "H" as "?". by eauto. }
-rewrite or_sep2. iDestruct "inv_ts" as "[resp_pred inv_ts]".
-wp_apply ("wp_f" with "[$]"). iIntros "%ts' (inv_ts' & inv)".
-case: ts' => [ts'|]; wp_pures; last first.
-{ wp_list.
-  wp_apply (Conn.wp_send with "[] [] [$conn]") => //.
-  { by rewrite /= public_TInt. }
-  { by iRight. }
-  iIntros "conn". wp_pures.
-  iApply "post". iModIntro. iLeft. by iFrame. }
-iDestruct "inv_ts'" as "(#p_ts' & inv_ts')".
-wp_apply (Conn.wp_send with "[] [] [inv_ts' resp_pred $conn]") => //.
-{ by iApply ctx_resp. }
-{ iDestruct "inv_ts'" as "[(_ & ? & _)|inv_ts']"; first by eauto.
-  iDestruct "resp_pred" as "[(_ & ? & _)|resp_pred]"; first by eauto.
-  iRight. iExists _. iFrame. }
-iIntros "conn". wp_pures. iApply "post". iModIntro.
-iLeft. by iFrame.
+iIntros "%Ξ (#N & #ctx & #wp) post". wp_lam. wp_pures.
+iApply wp_handle_gen; last by eauto.
+do 2![iSplit; eauto]. clear Ξ.
+iIntros "!> %t %Ξ !> (#p_t & inv_t & rel & inv) post".
+wp_pures.
+wp_apply ("wp" with "[$inv_t $inv]") => //.
+iIntros ([t'|]) "[ot' inv]"; wp_pures; last by iApply ("post" $! None); iFrame.
+iApply ("post" $! (Some (true, t'))). by iFrame.
 Qed.
 
 Lemma wp_handle_close Φ skI skR cs :
@@ -208,25 +269,62 @@ Lemma wp_handle_close Φ skI skR cs :
     impl.handle_close
   {{{ h, RET (repr h); wf_handler Φ skI skR cs h }}}.
 Proof.
-iIntros "%Ψ #ctx post".
-wp_apply Conn.wp_handle; last by eauto. clear Ψ.
-iPoseProof (ctx_close with "ctx") as "#?".
-iPoseProof (ctx_resp with "ctx") as "#?".
-iSplit => //.
-iIntros "!> %ts !> %Ψ (conn & inv & #p_ts & inv_ts) post".
-iDestruct "inv" as "(rel & inv)". wp_pures.
-iMod (release with "rel") as "#relS".
-iPoseProof (Conn.connected_released_session with "conn") as "#s_k".
-iAssert (|==> public (si_key cs))%I with "[inv_ts]" as ">#p_k".
-{ iDestruct "inv_ts" as "[?|[_ relC]]"; first by eauto.
-  iIntros "!>". iApply "s_k". by iSplit. }
-wp_pures. wp_list.
-wp_apply (Conn.wp_send with "[] [] [$conn]") => //.
-- by rewrite /= public_TInt.
-- by iLeft.
-iIntros "conn". wp_pures. wp_apply (Conn.wp_free with "[$conn]").
-iIntros "_". wp_pures. iApply "post".
-iModIntro. iFrame. iRight. by eauto.
+iIntros "%Ξ #ctx post".
+wp_apply wp_handle_gen; last by eauto.
+iSplit; first by iDestruct "ctx" as "[??]".
+iSplit; eauto. clear Ξ.
+iIntros "!> %t %Ξ !> (#p_t & #inv_t & rel & inv) post".
+iMod (release with "rel") as "#?".
+wp_pures. iApply ("post" $! (Some (false, _))). iFrame.
+iModIntro. iSplit; eauto.
+iDestruct "inv_t" as "[?|inv_t]"; eauto.
+iRight. by iSplit.
+Qed.
+
+Lemma wp_select Φ skI skR cs handlers :
+  {{{ ctx ∗
+      server_connected skI skR cs ∗
+      Φ ∗
+      [∗ list] h ∈ handlers, wf_handler Φ skI skR cs h }}}
+    impl.select (repr cs) (repr handlers)
+  {{{ ob, RET (repr ob);
+      match ob with
+      | Some false => Φ ∗ public (si_key cs)
+      | _ => Φ ∗ server_connected skI skR cs
+      end }}}.
+Proof.
+iIntros "%Ψ (#ctx & (conn & rel) & inv & #wp_handlers) post".
+wp_lam. wp_pures. iPoseProof "ctx" as "[??]".
+wp_apply (Conn.wp_recv with "[//] [$]").
+iIntros "%m (conn & #p_m & inv_m)". wp_pures.
+wp_apply (wp_handle_close Φ skI skR cs); eauto.
+iIntros "%h #wp_h". wp_list. wp_pures.
+iApply (wp_wand _ _ _ (λ v,
+  ∃ ob : option bool,
+    ⌜v = repr ob⌝ ∗
+    match ob with
+    | Some true => Φ ∗ server_connected skI skR cs
+    | Some false => Φ ∗ public (si_key cs)
+    | None => Φ ∗ server_connected skI skR cs ∗
+              (public (si_key cs) ∨ rpc_msg_pred skI skR cs Init m)
+    end) with "[rel inv conn inv_m] [post]")%I; last first.
+{ iIntros "% (% & -> & H)". iApply "post".
+  case: ob => [[]|]; eauto.
+  by iDestruct "H" as "(?&?&?)"; iFrame. }
+clear Ψ.
+wp_apply (wp_scan_list (wf_handler Φ skI skR cs) with "[]"); last first.
+{ iSplit => //=; eauto. iExists None. by iFrame. }
+iClear "wp_handlers wp_h". clear h.
+iIntros "!> %h %Ψ !> ((%ob & %e & inv) & #wp_h) post".
+case: ob => [[]|] //= in e *.
+iDestruct "inv" as "(inv & (conn & rel) & inv_m)".
+wp_pures. rewrite /wf_handler.
+iApply ("wp_h" with "[$conn $rel $inv_m $inv]") => //.
+iIntros "!> %ob H".
+have -> : repr ob = repr (((λ b : bool, #b) <$> ob)).
+  by case: ob => [[]|].
+iApply "post". iExists ob. iFrame.
+by case: ob => [[]|].
 Qed.
 
 Lemma wp_server Φ skI skR cs handlers :
@@ -238,23 +336,15 @@ Lemma wp_server Φ skI skR cs handlers :
 Proof.
 iLöb as "IH".
 iIntros "%Ψ (#ctx & conn & inv & #handlers) post".
-iDestruct "conn" as "(conn & rel)".
-iPoseProof (Conn.connected_keyE with "conn") as "#(-> & -> & _)".
-wp_rec. wp_pures. wp_apply (wp_handle_close Φ _ _ cs); eauto.
-iIntros "%hc #wp_hc". wp_list.
-iAssert ([∗ list] h ∈ (hc :: handlers), wf_handler Φ _ _ cs h)%I
-  as "#wp".
-{ rewrite /=; iSplit => //. eauto. }
-iClear "wp_hc". wp_bind (Conn.select _ _).
-iApply (wp_wand with "[inv conn rel]").
-{ wp_apply (Conn.wp_select with "wp [$conn $rel $inv]"). }
-iIntros "%res Hres".
-iDestruct "Hres" as "[(-> & Hres)|(-> & Hres)]".
-- iDestruct "Hres" as "(inv & conn & rel)". wp_pures.
-  wp_apply ("IH" with "[$inv $rel $conn]") => //.
-  by do !iSplit => //.
-- iDestruct "Hres" as "(inv & rel)". wp_pures.
-  iApply "post". by iFrame.
+wp_rec. wp_pures. wp_apply (wp_select with "[$conn inv]").
+{ by iFrame "#". }
+iIntros "%ob H". wp_pures.
+case: ob => [[]|]; wp_pures.
+- iDestruct "H" as "[inv server]".
+  by iApply ("IH" with "[$] post").
+- iDestruct "H" as "[inv #?]". iApply "post". by iFrame.
+- iDestruct "H" as "[inv server]".
+  by iApply ("IH" with "[$] post").
 Qed.
 
 Lemma wp_close skI skR cs :
@@ -263,29 +353,39 @@ Lemma wp_close skI skR cs :
   {{{ RET #(); public (si_key cs) }}}.
 Proof.
 iIntros "%Φ (#ctx & conn) post".
+iDestruct "ctx" as "[close ctx]".
 iDestruct "conn" as "(conn & rel & resp_pred)".
-iPoseProof (Conn.connected_keyE with "conn") as "#(-> & -> & _)".
-wp_lam. wp_pures. wp_list.
-iMod (release with "rel") as "#relC".
-iPoseProof (ctx_close with "[//]") as "#?".
-iPoseProof (ctx_resp with "[//]") as "#?".
+iMod (release with "rel") as "#rel".
+iAssert (|==>
+  (compromised_session Init cs ∨
+     resp_pred_token cs (rpcN.@"close") (TInt 0) ∗
+     resp_pred_token cs (rpcN.@"close") (TInt 0)))%I
+  with "[resp_pred]" as ">resp_pred".
+{ iDestruct "resp_pred" as "[#fail|(t1 & t2)]"; eauto.
+  iRight.
+  iApply (resp_pred_token_update with "t1 t2"). }
 rewrite or_sep2. iDestruct "resp_pred" as "[t1 t2]".
-wp_apply (Conn.wp_send with "[] [] [$conn t2]") => //.
-{ rewrite /= public_TInt. by eauto. }
-{ iDestruct "t2" as "[(_ & ? & _)|?]"; first by eauto.
-  iRight. by iFrame. }
-iIntros "conn". wp_pures.
-wp_apply (Conn.wp_recv with "[] [$]"); eauto.
-iIntros "%ts (conn & _ & inv)". wp_pure _ credit:"c".
-wp_pures. iApply wp_fupd.
-wp_apply (Conn.wp_free with "[$conn]"). iIntros "_".
-iApply "post".
-iDestruct "t1" as "[(_ & ? & _)|t1]"; eauto.
-iDestruct "inv" as "[#p_k|(% & t2 & inv)]"; eauto.
-iPoseProof (resp_pred_token_agree with "t1 t2") as "#E".
-iSpecialize ("E" $! ts). iMod (lc_fupd_elim_later_pers with "c E") as "{E} #E".
-iAssert False%I as "[]".
-by iRewrite "E".
+wp_lam. wp_lam. wp_pures. wp_tag.
+wp_apply (Conn.wp_send with "[] [] [$conn t2]"); eauto.
+{ by rewrite public_tag public_TInt. }
+{ iDestruct "t2" as "[(_ & ? & _)|?]"; first by eauto. iRight.
+  iExists _, _, _, _. iSplit => //. iFrame "#". by iFrame. }
+iIntros "conn". wp_pure _ credit:"c". wp_pures.
+wp_apply (Conn.wp_recv with "[] [$conn]"); eauto.
+iIntros "%t' (conn & p_t' & inv)".
+iAssert (|={⊤}=> public (si_key cs))%I with "[t1 inv c]" as ">#?".
+{ iDestruct "t1" as "[(_&?&_)|t1]"; eauto.
+  iDestruct "inv" as "[inv|inv]"; eauto.
+  iDestruct "inv" as "(%N' & %t₀ & %φ' & %ψ' & #N' & inv & t2)".
+  iPoseProof (resp_pred_token_agree with "t1 t2") as "[<- <-]".
+  iPoseProof (rpc_pred_agree with "close N'") as "[_ E]".
+  iSpecialize ("E" $! skI skR cs (TInt 0) t').
+  iMod (lc_fupd_elim_later_pers with "c E") as "{E} #E".
+  iRevert "inv".
+  iRewrite -"E". iIntros "[]". }
+wp_pures.
+wp_apply (Conn.wp_free with "[$conn]").
+iIntros "_". by iApply "post".
 Qed.
 
 End Proofs.
