examples/conn.v
@@ -8,6 +8,3 @@ Include cryptis.examples.conn.proofs.
 End Conn.
 
 Coercion Conn.cs_si : Conn.state >-> sess_info.
-Existing Instance Conn.repr_handler.
-Existing Instance Conn.persistent_wf_handler.
-#[global] Typeclasses Opaque Conn.wf_handler.
