examples/store/proofs/client/store.v
@@ -38,11 +38,11 @@ Proof.
 iIntros "#? #ctx #p_t1 #p_t2 !> %Φ [client mapsto] post".
 iDestruct "client" as "(conn & db)".
 iMod (store_call t2' with "db mapsto") as "(store & mapsto & waiting)".
-wp_lam. wp_pures. wp_list.
+wp_lam. wp_pures. wp_list. wp_term_of_list.
 iPoseProof (store_ctx_store with "[//]") as "?".
 iPoseProof (store_ctx_rpc_ctx with "[//]") as "?".
 wp_apply (RPC.wp_call with "[$conn $store]").
-{ do 4!iSplit => //=; first by eauto. }
+{ rewrite public_of_list. do 4!iSplit => //=; first by eauto. }
 iIntros "%ts' (conn & store & _)". wp_pures. iApply "post".
 iFrame. by iApply "waiting".
 Qed.
