examples/store/proofs/server/create.v
@@ -28,7 +28,7 @@ Ltac failure := iLeft; iFrame; eauto.
 
 Lemma wp_server_handle_create skI skR cs (vdb : val) :
   {{{ cryptis_ctx ∗ store_ctx }}}
-    RPC.handle (Tag $ dbN.@"create") (Server.handle_create (repr cs) vdb)
+    RPC.handle (Tag $ dbN.@"create") (Server.handle_create vdb)
   {{{ h, RET (repr h); server_handler skI skR cs vdb h }}}.
 Proof.
 iIntros "%Φ (#ctx & #ctx') post".
@@ -37,11 +37,13 @@ iPoseProof (store_ctx_rpc_ctx with "[//]") as "?".
 wp_lam. wp_pures.
 wp_apply RPC.wp_handle; last by eauto.
 do 2!iSplit => //. clear Φ.
-iIntros "!> %ts !> %Φ (#p_ts & inv_ts & %db & #p_db & db & ready) post".
+iIntros "!> %t !> %Φ (#p_ts & inv_ts & %db & #p_db & db & ready) post".
+wp_pures. wp_list_of_term t; wp_pures; last first.
+{ iApply ("post" $! None). by iFrame. }
 wp_list_match => [t1 t2 ->| ?]; wp_pures; last first.
-{ iApply ("post" $! None). iFrame.
-  iDestruct "inv_ts" as "[fail|inv_ts]"; eauto. }
-rewrite /=. iDestruct "p_ts" as "(p_t1 & p_t2 & _)".
+{ iApply ("post" $! None). by iFrame. }
+rewrite /= public_of_list /=.
+iDestruct "p_ts" as "(p_t1 & p_t2 & _)".
 wp_bind (AList.find _ _). iApply (AList.wp_find with "db") => //.
 iIntros "!> db". rewrite lookup_fmap.
 case db_t1: (db !! t1) => [t2'|]; wp_pures.
@@ -50,8 +52,8 @@ iMod (create_resp with "ready inv_ts") as "[ready inv_ts]".
 wp_bind (AList.insert _ _ _).
 iApply (AList.wp_insert with "db").
 iIntros "!> db". rewrite -fmap_insert. wp_pures.
-wp_list. wp_pures. iApply ("post" $! (Some _)).
-iModIntro. rewrite /= public_TInt. iFrame. iSplit => //.
+iApply ("post" $! (Some _)).
+iModIntro. rewrite /= public_TInt. iFrame.
 by iApply public_db_insert.
 Qed.
 
