examples/store/proofs/server/load.v
@@ -29,7 +29,7 @@ Ltac failure := iLeft; iFrame; eauto.
 
 Lemma wp_server_handle_load skI skR cs (vdb : val) :
   {{{ cryptis_ctx ∗ store_ctx  }}}
-    RPC.handle (Tag $ (dbN.@"load")) (Server.handle_load (repr cs) vdb)
+    RPC.handle (Tag $ (dbN.@"load")) (Server.handle_load vdb)
   {{{ h, RET (repr h); server_handler skI skR cs vdb h }}}.
 Proof.
 iIntros "%Φ (#? & #ctx) post".
@@ -38,16 +38,14 @@ iPoseProof (store_ctx_rpc_ctx with "ctx") as "?".
 wp_lam; wp_pures.
 wp_apply RPC.wp_handle; last by eauto.
 do 2!iSplit => //. clear Φ.
-iIntros "!> %ts !> %Φ (#p_ts & inv_ts & %db & #p_db & db & ready) post".
-wp_pures. wp_list_match => [t1 ->| ?]; wp_pures; last first.
-{ iApply ("post" $! None). by iFrame. }
+iIntros "!> %t1 !> %Φ (#p_t1 & inv_t1 & %db & #p_db & db & ready) post".
+wp_pures.
 wp_bind (AList.find _ _). iApply (AList.wp_find with "db") => //.
 iIntros "!> db". rewrite lookup_fmap.
-iMod (load_resp with "ready inv_ts") as "[ready inv_ts]".
+iMod (load_resp with "ready inv_t1") as "[ready inv_t1]".
 case db_t1: (db !! t1) => [t2'|]; wp_pures; last first.
 { iApply ("post" $! None). by iFrame. }
-wp_list. wp_pures. iModIntro.
-iApply ("post" $! (Some _)). iFrame. do !iSplit; eauto.
+iApply ("post" $! (Some _)). iFrame. iModIntro. iSplit => //.
 rewrite /public_db big_sepM_forall /=.
 by iDestruct ("p_db" $! t1 t2' with "[//]") as "[??]".
 Qed.
